Zkpc.lean
@@ -21,6 +21,7 @@ import Zkpc.Network.State
 import Zkpc.Network.Credential
 import Zkpc.Games.Frame
 import Zkpc.Games.FrameAudit
+import Zkpc.Games.FrameIdeal
 import Zkpc.Games.Coupling
 import Zkpc.Games.FlatInstance
 import Zkpc.Games.FullTicketInstance
